Benchmarks.lean
@@ -1,6 +1,7 @@
 import Benchmarks.WETH9.Correct
 import Benchmarks.Safe.Correct
 import Benchmarks.UniswapV3Pool.Correct
+import Benchmarks.UniswapV2Router02.Correct
 import Benchmarks.Dss.Dai.Correct
 import Benchmarks.Dss.Jug.Correct
 import Benchmarks.Dss.Vat.Correct
